TypedAssembly.lean
@@ -1,4 +1,3 @@
 -- This module serves as the root of the `TypedAssembly` library.
 -- Import modules here that should be built as part of the library.
 import «TypedAssembly».Basic
-import «TypedAssembly».LambdaF
