TypedAssembly/LambdaF/TermEnv.lean
@@ -3,7 +3,7 @@ import «TypedAssembly».LambdaF.Typ
 inductive Ctx : Ctxt → Type where
   | nil       : Ctx Ø
   | snoc_kind : Ctx Δ → ∀ j, Ctx (Δ ,⋆ j)
-  | snoc_typ  : Ctx Δ → Δ ⊢⋆ ⋆ → Ctx Δ
+  | snoc_typ  : Ctx Δ → Δ ⊢F⋆ ⋆ → Ctx Δ
 
 namespace Ctx
   infixl:50 " ,, " => Ctx.snoc_typ
@@ -12,10 +12,10 @@ namespace Ctx
 end Ctx
 open Ctx
 
-inductive Lookup : Ctx Δ → Δ ⊢⋆ ⋆ → Type where
-  | here  {Γ : Ctx Δ} {t : Δ ⊢⋆ ⋆}     : Lookup (Γ ,, t) t
-  | there {Γ : Ctx Δ} {t₁ t₂ : Δ ⊢⋆ ⋆} : Lookup Γ t₁ → Lookup (Γ ,, t₂) t₁
-  | move  {Γ : Ctx Δ} {t : Δ ⊢⋆ ⋆} {k} : Lookup Γ t →
+inductive Lookup : Ctx Δ → Δ ⊢F⋆ ⋆ → Type where
+  | here  {Γ : Ctx Δ} {t : Δ ⊢F⋆ ⋆}     : Lookup (Γ ,, t) t
+  | there {Γ : Ctx Δ} {t₁ t₂ : Δ ⊢F⋆ ⋆} : Lookup Γ t₁ → Lookup (Γ ,, t₂) t₁
+  | move  {Γ : Ctx Δ} {t : Δ ⊢F⋆ ⋆} {k} : Lookup Γ t →
                                          Lookup (Γ ,,⋆ k) (weakenτ t)
 deriving Repr
 
@@ -24,6 +24,6 @@ namespace Lookup
 end Lookup
 open Lookup
 
-def conv_ni {Δ Γ} {t₁ t₂ : Δ ⊢⋆ ⋆} : t₁ = t₂ → (Γ ∋ t₁) → Γ ∋ t₂
+def conv_ni {Δ Γ} {t₁ t₂ : Δ ⊢F⋆ ⋆} : t₁ = t₂ → (Γ ∋ t₁) → Γ ∋ t₂
   | rfl, a => a
 
